Switched to swap-pi and swap-sigma

Gt3/HasTy/Basic.lean
@@ -9,9 +9,9 @@ inductive Ctx.HasTy : Ctx → Tm 0 → Tm 0 → Prop
   | eqn {Γ} {A a b : Tm 0} {ℓ : ULevel}
     (ha : HasTy Γ A a) (hb : HasTy Γ A b)
     : HasTy Γ (.univ ℓ) (.eqn a b)
-  | pi {Γ} {A : Tm 0} {B : Tm 1} {ℓ m n : ULevel} {L : Finset String}
+  | pi' {Γ} {A : Tm 0} {B : Tm 1} {ℓ m n : ULevel} {L : Finset String}
     (hA : HasTy Γ (.univ m) A) (hB : ∀ x ∉ L, HasTy (Γ.cons x A) (.univ n) (B.open x))
-    (hm : m ≤ ℓ) (hn : n ≤ ℓ) (hℓ : 1 ≤ ℓ)
+    (hm : m ≤ ℓ) (hn : n ≤ ℓ)
     : HasTy Γ (.univ ℓ) (.pi A B)
   | abs' {Γ} {A : Tm 0} {B b : Tm 1} {m n : ULevel} {L : Finset String}
     (hA : HasTy Γ (.univ m) A)
@@ -24,9 +24,9 @@ inductive Ctx.HasTy : Ctx → Tm 0 → Tm 0 → Prop
     (hf : HasTy Γ (A.pi B) f) (ha : HasTy Γ A a)
     (hBa : TyEq Γ (B.lst a) Ba)
     : HasTy Γ Ba (f.app a)
-  | sigma {Γ} {A : Tm 0} {B : Tm 1} {ℓ m n : ULevel} {L : Finset String}
+  | sigma' {Γ} {A : Tm 0} {B : Tm 1} {ℓ m n : ULevel} {L : Finset String}
     (hA : HasTy Γ (.univ m) A) (hB : ∀ x ∉ L, HasTy (Γ.cons x A) (.univ n) (B.open x))
-    (hm : m ≤ ℓ) (hn : n ≤ ℓ) (hℓ : 1 ≤ ℓ)
+    (hm : m ≤ ℓ) (hn : n ≤ ℓ)
     : HasTy Γ (.univ ℓ) (.sigma A B)
   | pair' {Γ} {A a b : Tm 0} {B : Tm 1} {m n : ULevel} {L : Finset String}
     (hA : HasTy Γ (.univ m) A) (hB : ∀ x ∉ L, HasTy (Γ.cons x A) (.univ n) (B.open x))
